\section{Cross-section $2 \rightarrow 1$ in terms of decay width}

It is possible to express corss-section $2 \rightarrow 1$ in terms of decay width $1 \rightarrow 2$. We use center of mass frame. For decay width there is a well known expression~\cite{pdg}:

\begin{align}
    \dd{\Gamma} = \frac{\vec{p}_{c.m.}}{32 \pi^2 m^2} \abs{\Mcal}^2 \dd{\Omega}
\end{align}

As cross-section $2 \rightarrow 1$ is unusual, we provide complete derivation from first principles:

\begin{align}
        &\sigma(2 \rightarrow 1) = \sum_{\lambda_f} \int \lips{\vec{p}_f} \frac{(2\pi)^4 \delta^{(4)}(p_i + p_\gamma - p_f)}{(2 \Ep{i}) (2 \Ep{\gamma}) j} \abs{\Mcal_{\lambda_i \lambda_\gamma, \lambda_f}(\vec{p}_i + \vec{p}_\gamma \rightarrow \vec{p}_f)}^2 = \\
        &= \frac{2\pi}{8 \Ep{f} \Ep{i} \Ep{\gamma} j} \delta(\Ep{i} + \Ep{\gamma} - \Ep{f}) \sum_{\lambda_f} \abs{\Mcal_{\lambda_i \lambda_\gamma, \lambda_f}}^2 = \left| \Ep{i} \Ep{\gamma} j = E_{c.m.} \abs{\vec{p}_{c.m.}} \right| = \\
        &= \left| \Ep{f} = E_{c.m.} = m_f \right| = \frac{\pi}{4 m_f^2 \abs{\vec{p}_{c.m.}}} \delta(\sqrt{s} - m_f) \sum_{\lambda_f} \abs{\Mcal_{\lambda_i \lambda_\gamma, \lambda_f}}^2 = \\
        &= \frac{2 \pi \sqrt{s}}{4 m_f^2 \abs{\vec{p}_{c.m.}}} \delta(s - m_f^2) \sum_{\lambda_f} \abs{\Mcal_{\lambda_i \lambda_\gamma, \lambda_f}}^2 = \left| \abs{\vec{p}_{c.m.}} = \frac{m_f^2 - m_i^2}{2 m_f} \right| =\\
        &= \frac{\pi}{m_f^2 - m_i^2} \delta(s - m_f^2) \sum_{\lambda_f} \abs{\Mcal_{\lambda_i \lambda_\gamma, \lambda_f}}^2
\end{align}

\begin{align}
        &\Gamma(1 \rightarrow 2) =  \frac{m_f^2 - m_i^2}{64 \pi^2 m_f^3} \int \dd{\Omega} \abs{\Mcal_{\lambda_f, \lambda_i \lambda_\gamma}(\vec{p}_f \rightarrow \vec{p}_i + \vec{p}_\gamma)}^2 = \\
        &= \frac{m_f^2 - m_i^2}{64 \pi^2 m_f^3} \int \dd{\Omega} \sum_{\lambda_f^{\prime \star} \lambda_f^{\prime}} D^{J_f \star}_{\lambda^{\prime \star}_f \lambda_f}(\Omega) D^{J_f}_{\lambda^{\prime}_f \lambda_f}(\Omega) \Mcal^\star_{\lambda^{\prime \star}_f, \lambda_i \lambda_\gamma} \Mcal_{\lambda_f, \lambda_i \lambda_\gamma} = \\
        &= \left| \int \dd{\Omega}D^{J_f \star}_{\lambda^{\prime \star}_f \lambda_f}(\Omega) D^{J_f}_{\lambda^{\prime}_f \lambda_f}(\Omega) = \frac{4 \pi}{2J_f + 1} \delta_{\lambda_f^\prime, \lambda_f^{\prime \star}}  \right| = \\
        &= \frac{m_f^2 - m_i^2}{16 \pi m_f^3} \frac{1}{2J_f + 1} \sum_{\lambda_f} \abs{\Mcal_{\lambda_f, \lambda_i \lambda_\gamma}}^2
\end{align}

Finally, we can re-express cross-section in terms of decay width:

\begin{align} \label{eq:app:crsc-dw}
    \sigma = \frac{16 \pi^2 m_f^3}{(m_f^2 - m_i^2)^2} (2J_f + 1) \Gamma \delta(s - m_f^2)
\end{align}

\paragraph{Subthreshold pole} Here we assumed final states being heavier then initial vector meson. If this is not true we get a modified expression for decay width, because we still want to keep it physical. Natural physical value corresponding to such a process is decay of vector meson into the bound state with photon emission. Actually, when comparing to previous formula it means interchanging of $m_i$ width $m_f$, $\lambda_i$ with $\lambda_f$, and $J_f$ with $J_i$:

\begin{align}
        \Gamma = \frac{m_i^2 - m_f^2}{16 \pi m_i^3} \frac{1}{2J_i + 1} \sum_{\lambda_i} \abs{\Mcal_{\lambda_i, \lambda_f \lambda_\gamma}}^2 \\
        \sigma = \frac{\pi}{m_f^2 - m_i^2} \delta(s - m_f^2) \sum_{\lambda_f} \abs{\Mcal_{\lambda_i \lambda_\gamma, \lambda_f}}^2
\end{align}

At the first sight, one can notice that matrix element now contributes to decay width in a completely different way comparing to cross-section. We can reduce this difference by making use of parity, time reversal and crossing symmetry:

\begin{align}
    &\text{Crossing $i \leftrightarrow r$:}\qquad &\sum_{\lambda_i} \abs{\Mcal_{\lambda_f, \lambda_\gamma \lambda_i}}^2 \rightarrow \sum_{\lambda_i} \abs{\Mcal_{-\lambda_i, \lambda_\gamma (-\lambda_f)}}^2 \\
    &\mathcal{P}:\qquad &\sum_{\lambda_i} \abs{\Mcal_{-\lambda_i, \lambda_\gamma (-\lambda_f)}}^2 \rightarrow \sum_{\lambda_i} \abs{\Mcal_{\lambda_i, (-\lambda_\gamma) \lambda_f}}^2\\
    &\mathcal{T}:\qquad &\sum_{\lambda_i} \abs{\Mcal_{\lambda_i, (-\lambda_\gamma) \lambda_f}}^2 \rightarrow \abs{\Mcal_{(-\lambda_\gamma) \lambda_f, \lambda_i}}^2
\end{align}

We acquired flipping of photon helicity in comparison to matrix element contributing to the cross-section. In the language of total helicities it corresponds to flipping $\Lambda=0$ and $\Lambda=2$. This corresponds to the flipping of sign near the subthreshold terms ($\sigma(2) - \sigma(0) \rightarrow \Gamma(0) - \Gamma(2)$):

\begin{align} \label{eq:app:crsc-dw-subthr}
    \sigma = -\frac{16 \pi^2 m_f^3}{(m_i^2 - m_f^2)^2} (2J_i + 1) \Gamma \delta(s - m_f^2)
\end{align}
